New patterns for new buffers. Fix post of upd

ulib/LowStar.Buffer.fst
@@ -190,6 +190,21 @@ let as_addr_disjoint #a1 #a2 b1 b2 = ()
 
 let gsub_disjoint #a b i1 len1 i2 len2 = ()
 
+let pointer_distinct_sel_disjoint #a b1 b2 h =
+  if frameOf b1 = frameOf b2 && as_addr b1 = as_addr b2
+  then begin
+    let t1 = vec a (U32.v (Buffer?.max_length b1)) in
+    let t2 = vec a (U32.v (Buffer?.max_length b2)) in
+    let r1 : HST.reference t1 = Buffer?.content b1 in
+    let r2' : HST.reference t2 = Buffer?.content b2 in
+    assert (Buffer?.max_length b1 == Buffer?.max_length b2);
+    assert (t1 == t2);
+    let r2 : HS.reference t1 = r2' in
+    HS.reference_distinct_sel_disjoint h (Buffer?.content b1) r2
+  end
+  else ()
+
+
 (* Untyped view of buffers, used only to implement the generic modifies clause. DO NOT USE in client code. *)
 
 noeq
